factor out pcond in basic symbolic execution for swap example

examples/riscv/swap/swap_symb_execScript.sml
@@ -9,29 +9,13 @@ open swapTheory;
 
 val _ = new_theory "swap_symb_exec";
 
-val bprog_tm = (snd o dest_eq o concl) bir_swap_prog_def;
-
 (* ........................... *)
 
 val birs_state_init_lbl = (snd o dest_eq o concl o EVAL) ``bir_block_pc (BL_Address (Imm64 0x00w))``;
+
 val birs_stop_lbls = [(snd o dest_eq o concl o EVAL) ``bir_block_pc (BL_Address (Imm64 0x14w))``];
 
-(* +++++++++++++++++++++++++++++++++++++++++++++++++++++++++++ *)
-Definition riscv_vars_def:
-  riscv_vars = APPEND (bmr_vars riscv_bmr) (bmr_temp_vars riscv_bmr)
-End
-
-Definition birenvtyl_riscv_def:
-  birenvtyl_riscv = MAP BVarToPair riscv_vars
-End
-(* +++++++++++++++++++++++++++++++++++++++++++++++++++++++++++ *)
-
-
-
-(* TODO: add a sanity check here that all the variables of the program are included in birenvtyl! *)
-
-val mem_addrs_aligned_prog_disj_x10 = ``
-  BExp_BinExp BIExp_And
+val mem_addrs_aligned_prog_disj_x10 = ``BExp_BinExp BIExp_And
     (BExp_Aligned Bit64 3 (BExp_Den (BVar "sy_x10" (BType_Imm Bit64))))
     (BExp_BinExp BIExp_And
       (BExp_BinPred BIExp_LessOrEqual
@@ -39,10 +23,9 @@ val mem_addrs_aligned_prog_disj_x10 = ``
         (BExp_Den (BVar "sy_x10" (BType_Imm Bit64))))
       (BExp_BinPred BIExp_LessThan
         (BExp_Den (BVar "sy_x10" (BType_Imm Bit64)))
-        (BExp_Const (Imm64 0x100000000w)))
-    )``;
-val mem_addrs_aligned_prog_disj_x11 = ``
-  BExp_BinExp BIExp_And
+        (BExp_Const (Imm64 0x100000000w))))``;
+
+val mem_addrs_aligned_prog_disj_x11 = ``BExp_BinExp BIExp_And
     (BExp_Aligned Bit64 3 (BExp_Den (BVar "sy_x11" (BType_Imm Bit64))))
     (BExp_BinExp BIExp_And
       (BExp_BinPred BIExp_LessOrEqual
@@ -50,16 +33,47 @@ val mem_addrs_aligned_prog_disj_x11 = ``
         (BExp_Den (BVar "sy_x11" (BType_Imm Bit64))))
       (BExp_BinPred BIExp_LessThan
         (BExp_Den (BVar "sy_x11" (BType_Imm Bit64)))
-        (BExp_Const (Imm64 0x100000000w)))
-    )``;
+        (BExp_Const (Imm64 0x100000000w))))``;
 
+val birs_pcond = ``BExp_BinExp
+ BIExp_And
+  ^mem_addrs_aligned_prog_disj_x10
+  ^mem_addrs_aligned_prog_disj_x11``;
+
+(* +++++++++++++++++++++++++++++++++++++++++++++++++++++++++++ *)
+
+Definition swap_prog_vars_def:
+  swap_prog_vars = [
+    BVar "MEM8" (BType_Mem Bit64 Bit8);
+    BVar "x15" (BType_Imm Bit64);
+    BVar "x14" (BType_Imm Bit64);
+    BVar "x11" (BType_Imm Bit64);
+    BVar "x10" (BType_Imm Bit64);
+    BVar "x1" (BType_Imm Bit64)
+  ]
+End
+
+Theorem swap_prog_vars_thm:
+  set swap_prog_vars = bir_vars_of_program (bir_swap_prog : 'observation_type bir_program_t)
+Proof
+  SIMP_TAC (std_ss++HolBASimps.VARS_OF_PROG_ss++pred_setLib.PRED_SET_ss)
+   [bir_swap_prog_def, swap_prog_vars_def] >>
+  EVAL_TAC
+QED
+
+Definition swap_birenvtyl_def:
+  swap_birenvtyl = MAP BVarToPair swap_prog_vars
+End
+
+(* +++++++++++++++++++++++++++++++++++++++++++++++++++++++++++ *)
 
 val birs_state_init = ``<|
   bsst_pc       := ^birs_state_init_lbl;
-  bsst_environ  := bir_senv_GEN_list birenvtyl_riscv;
+  bsst_environ  := bir_senv_GEN_list swap_birenvtyl;
   bsst_status   := BST_Running;
-  bsst_pcond    := BExp_BinExp BIExp_And ^mem_addrs_aligned_prog_disj_x10 ^mem_addrs_aligned_prog_disj_x11
+  bsst_pcond    := ^birs_pcond
 |>``;
+
 (* TODO: probably need this later in the path condition: 
   ``BExp_UnaryExp BIExp_Not (BExp_Den (BVar "ModeHandler" BType_Bool))``;
 
@@ -71,22 +85,24 @@ val birs_state_init = ``<|
 
 BExp_Const (Imm1 1w)
 
- *)
+*)
+
 (* ........................... *)
+
+val bprog_tm = (snd o dest_eq o concl) bir_swap_prog_def;
 
 val birs_rule_STEP_thm = birs_rule_STEP_prog_fun (bir_prog_has_no_halt_fun bprog_tm);
 val birs_rule_SUBST_thm = birs_rule_SUBST_prog_fun bprog_tm;
 val birs_rule_STEP_fun_spec = (birs_rule_SUBST_trysimp_const_add_subst_fun birs_rule_SUBST_thm o birs_rule_tryjustassert_fun true o birs_rule_STEP_fun birs_rule_STEP_thm bprog_tm);
+
 (* now the composition *)
 val birs_rule_SEQ_thm = birs_rule_SEQ_prog_fun bprog_tm;
 val birs_rule_SEQ_fun_spec = birs_rule_SEQ_fun birs_rule_SEQ_thm;
 (* ........................... *)
 
-
 val single_step_A_thm = birs_rule_STEP_fun_spec birs_state_init;
+
 (* ........................... *)
-
-
 
 (* and also the sequential composition *)
 val birs_rule_STEP_SEQ_thm = MATCH_MP birs_rulesTheory.birs_rule_STEP_SEQ_gen_thm (bir_prog_has_no_halt_fun bprog_tm);
@@ -97,7 +113,6 @@ val birs_rule_STEP_SEQ_fun_spec = birs_rule_STEP_SEQ_fun (birs_rule_SUBST_thm, b
 val tree = build_tree (birs_rule_STEP_fun_spec, birs_rule_SEQ_fun_spec, birs_rule_STEP_SEQ_fun_spec) single_step_A_thm birs_stop_lbls;
 val _ = print "done building the tree\n";
 *)
-
 val _ = print "now reducing it to one sound structure\n";
 
 val timer = bir_miscLib.timer_start 0;
